theories/lang/cpp/logic/pred.v
@@ -57,7 +57,8 @@ Module Type CPP_LOGIC
     Context `{Σ : cpp_logic}.
 
     (**
-      [_valid_ptr vt p] is a persistent assertion that [p] is a _valid pointer_, that is:
+      [_valid_ptr vt ty p] is a persistent assertion that [p] is a _valid pointer_,
+      at type [ty] that is:
       - [p] can point to a function or a (possibly dead) object [o]
       - if [vt = Relaxed], [p] can be nullptr, or past-the-end of a (possibly dead) object [o].
       In particular, [_valid_ptr vt p] prevents producing [p] by incrementing
@@ -94,21 +95,21 @@ Module Type CPP_LOGIC
       http://www.open-std.org/jtc1/sc22/wg14/www/docs/n2369.pdf for
       discussion in the context of the C standard.
     *)
-    Parameter _valid_ptr : forall (vt : validity_type), ptr -> mpred.
+    Parameter _valid_ptr : forall (vt : validity_type), type -> ptr -> mpred.
     (* strict validity (not past-the-end) *)
     Notation strict_valid_ptr := (_valid_ptr Strict).
     (* validity (past-the-end allowed) *)
     Notation valid_ptr := (_valid_ptr Relaxed).
 
-    Axiom _valid_ptr_persistent : forall b p, Persistent (_valid_ptr b p).
-    Axiom _valid_ptr_affine : forall b p, Affine (_valid_ptr b p).
-    Axiom _valid_ptr_timeless : forall b p, Timeless (_valid_ptr b p).
+    Axiom _valid_ptr_persistent : forall b ty p, Persistent (_valid_ptr b ty p).
+    Axiom _valid_ptr_affine : forall b ty p, Affine (_valid_ptr b ty p).
+    Axiom _valid_ptr_timeless : forall b ty p, Timeless (_valid_ptr b ty p).
     #[global] Existing Instances _valid_ptr_persistent _valid_ptr_affine _valid_ptr_timeless.
 
-    Axiom valid_ptr_nullptr : |-- valid_ptr nullptr.
-    Axiom not_strictly_valid_ptr_nullptr : strict_valid_ptr nullptr |-- False.
-    Axiom strict_valid_valid : forall p,
-      strict_valid_ptr p |-- valid_ptr p.
+    Axiom valid_ptr_nullptr : forall ty, |-- valid_ptr ty nullptr.
+    Axiom not_strictly_valid_ptr_nullptr : forall ty, strict_valid_ptr ty nullptr |-- False.
+    Axiom strict_valid_valid : forall p ty,
+      strict_valid_ptr ty p |-- valid_ptr ty p.
 
     (** Formalizes the notion of "provides storage",
     http://eel.is/c++draft/intro.object#def:provides_storage *)
@@ -175,8 +176,8 @@ Module Type CPP_LOGIC
     Axiom live_alloc_id_timeless : forall aid, Timeless (live_alloc_id aid).
     #[global] Existing Instance live_alloc_id_timeless.
 
-    Axiom valid_ptr_alloc_id : forall p,
-      valid_ptr p |-- [| is_Some (ptr_alloc_id p) |].
+    Axiom valid_ptr_alloc_id : forall p ty,
+      valid_ptr ty p |-- [| is_Some (ptr_alloc_id p) |].
 
     (** This pointer is from a live allocation; this does not imply
     [_valid_ptr], because even overflowing offsets preserve the allocation ID.
@@ -243,7 +244,8 @@ Module Type CPP_LOGIC
     #[global] Declare Instance identity_cfractional σ this mdc : CFractional1 (identity this mdc).
     #[global] Declare Instance identity_cfrac_valid {σ} cls path : CFracValid1 (identity cls path).
     #[global] Declare Instance identity_timeless : Timeless5 (@identity).
-    #[global] Declare Instance identity_strict_valid σ this mdc q p : Observe (strict_valid_ptr p) (identity this mdc q p).
+    #[global] Declare Instance identity_strict_valid σ this mdc q p
+      : Observe (strict_valid_ptr (Tnamed this) p) (identity this mdc q p).
 
     (** cpp2v-core#194: Agreement? *)
 
@@ -297,23 +299,23 @@ Module Type CPP_LOGIC
       Axiom ctor_at_live   : forall f p,   ctor_at f p |-- live_ptr p.
       Axiom dtor_at_live   : forall f p,   dtor_at f p |-- live_ptr p.
 
-      Axiom code_at_strict_valid   : forall f p,   code_at f p |-- strict_valid_ptr p.
-      Axiom method_at_strict_valid : forall f p, method_at f p |-- strict_valid_ptr p.
-      Axiom ctor_at_strict_valid   : forall f p,   ctor_at f p |-- strict_valid_ptr p.
-      Axiom dtor_at_strict_valid   : forall f p,   dtor_at f p |-- strict_valid_ptr p.
+      Axiom code_at_strict_valid   : forall f p,   code_at f p |-- strict_valid_ptr (type_of_value $ Ofunction f) p.
+      Axiom method_at_strict_valid : forall f p, method_at f p |-- strict_valid_ptr (type_of_value $ Omethod f) p.
+      Axiom ctor_at_strict_valid   : forall f p,   ctor_at f p |-- strict_valid_ptr (type_of_value $ Oconstructor f) p.
+      Axiom dtor_at_strict_valid   : forall f p,   dtor_at f p |-- strict_valid_ptr (type_of_value $ Odestructor f) p.
 
     End with_genv.
 
-    Axiom offset_pinned_ptr_pure : forall σ o z va p,
+    Axiom offset_pinned_ptr_pure : forall σ ty o z va p,
       eval_offset σ o = Some z ->
       ptr_vaddr p = Some va ->
-      valid_ptr (p ,, o) |--
+      valid_ptr ty (p ,, o) |--
       [| ptr_vaddr (p ,, o) = Some (Z.to_N (Z.of_N va + z)) |].
 
-    Axiom offset_inv_pinned_ptr_pure : forall σ o z va p,
+    Axiom offset_inv_pinned_ptr_pure : forall σ ty o z va p,
       eval_offset σ o = Some z ->
       ptr_vaddr (p ,, o) = Some va ->
-      valid_ptr (p ,, o) |--
+      valid_ptr ty (p ,, o) |--
       [| 0 <= Z.of_N va - z |]%Z **
       [| ptr_vaddr p = Some (Z.to_N (Z.of_N va - z)) |].
 
@@ -321,9 +323,9 @@ Module Type CPP_LOGIC
       Observe [| same_address storage_ptr obj_ptr |] (provides_storage storage_ptr obj_ptr ty).
 
     Axiom provides_storage_valid_storage_ptr : forall storage_ptr obj_ptr aty,
-      Observe (valid_ptr storage_ptr) (provides_storage storage_ptr obj_ptr aty).
+      Observe (valid_ptr Tbyte storage_ptr) (provides_storage storage_ptr obj_ptr aty).
     Axiom provides_storage_valid_obj_ptr : forall storage_ptr obj_ptr aty,
-      Observe (valid_ptr obj_ptr) (provides_storage storage_ptr obj_ptr aty).
+      Observe (∃ ty, valid_ptr ty obj_ptr) (provides_storage storage_ptr obj_ptr aty).
 
     #[global] Existing Instances provides_storage_same_address
       provides_storage_valid_storage_ptr provides_storage_valid_obj_ptr.
@@ -399,10 +401,10 @@ Module Type CPP_LOGIC
     Recall that [type_ptr] and [strict_valid_ptr] don't include
     past-the-end pointers... *)
     Axiom type_ptr_strict_valid : forall resolve ty p,
-      type_ptr ty p |-- strict_valid_ptr p.
+      type_ptr ty p |-- strict_valid_ptr ty p.
     (** Hence they can be incremented into (possibly past-the-end) valid pointers. *)
     Axiom type_ptr_valid_plus_one : forall resolve ty p,
-      type_ptr ty p |-- valid_ptr (p ,, o_sub resolve ty 1).
+      type_ptr ty p |-- valid_ptr ty (p ,, o_sub resolve ty 1).
 
     (* When [p] is a [ptr] to a C++ object of type [ty], [p] is /also/ a pointer
        to the "object representation" of [ty] - which consists of "the sequence
@@ -553,8 +555,8 @@ Module Type CPP_LOGIC
      Validity is necessary: the C++ expression [(char * )p - (uintptr_t) p]
      produces an invalid pointer with address 0, which is not [nullptr] because
      it preserves the provenance of [p]. *)
-    Axiom same_address_eq_null : forall p tv,
-      _valid_ptr tv p |--
+    Axiom same_address_eq_null : forall p ty tv,
+      _valid_ptr tv ty p |--
       [| same_address p nullptr <-> p = nullptr |].
 
     (**
@@ -614,12 +616,12 @@ Module Type VALID_PTR_AXIOMS
   Section with_cpp.
     Context `{cpp_logic} {σ : genv}.
 
-    Axiom invalid_ptr_invalid : forall vt,
-      _valid_ptr vt invalid_ptr |-- False.
+    Axiom invalid_ptr_invalid : forall vt ty,
+      _valid_ptr vt ty invalid_ptr |-- False.
 
     (** Justified by [https://eel.is/c++draft/expr.add#4.1]. *)
     Axiom _valid_ptr_nullptr_sub_false : forall vt ty (i : Z) (_ : i <> 0),
-      _valid_ptr vt (nullptr ,, o_sub σ ty i) |-- False.
+      _valid_ptr vt ty (nullptr ,, o_sub σ ty i) |-- False.
     (*
     TODO Controversial; if [f] is the first field, [nullptr->f] or casts relying on
     https://eel.is/c++draft/basic.compound#4 might invalidate this.
@@ -639,8 +641,8 @@ Module Type VALID_PTR_AXIOMS
     *)
     Axiom strict_valid_ptr_sub : ∀ (i j k : Z) p ty vt1 vt2,
       (i <= j < k)%Z ->
-      _valid_ptr vt1 (p ,, o_sub σ ty i) |--
-      _valid_ptr vt2 (p ,, o_sub σ ty k) -* strict_valid_ptr (p ,, o_sub σ ty j).
+      _valid_ptr vt1 ty (p ,, o_sub σ ty i) |--
+      _valid_ptr vt2 ty (p ,, o_sub σ ty k) -* strict_valid_ptr ty (p ,, o_sub σ ty j).
 
     (** XXX: this axiom is convoluted but
     TODO: The intended proof of [strict_valid_ptr_field_sub] (and friends) is that
@@ -651,11 +653,11 @@ Module Type VALID_PTR_AXIOMS
     *)
     Axiom strict_valid_ptr_field_sub : ∀ (p : ptr) ty (i : Z) f vt,
       (0 < i)%Z ->
-      _valid_ptr vt (p ,, o_field σ f ,, o_sub σ ty i) |-- strict_valid_ptr (p ,, o_field σ f).
+      _valid_ptr vt ty (p ,, o_field σ f ,, o_sub σ ty i) |-- strict_valid_ptr ty (p ,, o_field σ f).
 
     (* TODO: can we deduce that [p] is strictly valid? *)
-    Axiom _valid_ptr_field : ∀ p f vt,
-      _valid_ptr vt (p ,, o_field σ f) |-- _valid_ptr vt p.
+    Axiom _valid_ptr_field : ∀ p f ty vt,
+      _valid_ptr vt ty (p ,, o_field σ f) |-- _valid_ptr vt (Tnamed f.(f_type)) p.
     (* TODO: Pointers to fields can't be past-the-end, right?
     Except 0-size arrays. *)
     (* Axiom strict_valid_ptr_field : ∀ p f,
@@ -672,16 +674,16 @@ Module Type VALID_PTR_AXIOMS
     (* We're ignoring virtual inheritance here, since we have no plans to
     support it for now, but this might hold there too. *)
     Axiom o_base_directly_derives : forall p base derived,
-      strict_valid_ptr (p ,, o_base σ derived base) |--
+      strict_valid_ptr (Tnamed base) (p ,, o_base σ derived base) |--
       [| directly_derives σ derived base |].
 
     Axiom o_derived_directly_derives : forall p base derived,
-      strict_valid_ptr (p ,, o_derived σ base derived) |--
+      strict_valid_ptr (Tnamed derived) (p ,, o_derived σ base derived) |--
       [| directly_derives σ derived base |].
 
     (* TODO: maybe add a validity of offsets to allow stating this more generally. *)
     Axiom valid_o_sub_size : forall p ty i vt,
-      _valid_ptr vt (p ,, o_sub σ ty i) |-- [| is_Some (size_of σ ty) |].
+      _valid_ptr vt ty (p ,, o_sub σ ty i) |-- [| is_Some (size_of σ ty) |].
 
     Axiom type_ptr_o_base : forall derived base p,
       class_derives derived [base] ->
@@ -707,13 +709,13 @@ Declare Module Export VALID_PTR : VALID_PTR_AXIOMS PTRS_INTF_AXIOM VALUES_INTF_A
 Section valid_ptr_code.
   Context `{Σ : cpp_logic} {σ : genv} (tu : translation_unit).
 
-  Lemma code_at_valid   : forall f p,   code_at _ tu f p |-- valid_ptr p.
+  Lemma code_at_valid   : forall f p,   code_at _ tu f p |-- valid_ptr (type_of_value $ Ofunction f) p.
   Proof. intros. rewrite code_at_strict_valid; apply strict_valid_valid. Qed.
-  Lemma method_at_valid : forall f p, method_at _ tu f p |-- valid_ptr p.
+  Lemma method_at_valid : forall f p, method_at _ tu f p |-- valid_ptr (type_of_value $ Omethod f) p.
   Proof. intros. rewrite method_at_strict_valid; apply strict_valid_valid. Qed.
-  Lemma ctor_at_valid   : forall f p,   ctor_at _ tu f p |-- valid_ptr p.
+  Lemma ctor_at_valid   : forall f p,   ctor_at _ tu f p |-- valid_ptr (type_of_value $ Oconstructor f) p.
   Proof. intros. rewrite ctor_at_strict_valid; apply strict_valid_valid. Qed.
-  Lemma dtor_at_valid   : forall f p,   dtor_at _ tu f p |-- valid_ptr p.
+  Lemma dtor_at_valid   : forall f p,   dtor_at _ tu f p |-- valid_ptr (type_of_value $ Odestructor f) p.
   Proof. intros. rewrite dtor_at_strict_valid; apply strict_valid_valid. Qed.
 End valid_ptr_code.
 
@@ -721,7 +723,7 @@ Section pinned_ptr_def.
   Context `{Σ : cpp_logic}.
 
   Definition exposed_ptr_def p : mpred :=
-    valid_ptr p ** ∃ aid, [| ptr_alloc_id p = Some aid |] ** exposed_aid aid.
+    (∃ ty, valid_ptr ty p) ** ∃ aid, [| ptr_alloc_id p = Some aid |] ** exposed_aid aid.
   Definition exposed_ptr_aux : seal exposed_ptr_def. Proof. by eexists. Qed.
   Definition exposed_ptr := exposed_ptr_aux.(unseal).
   Definition exposed_ptr_eq : exposed_ptr = _ := exposed_ptr_aux.(seal_eq).
@@ -735,36 +737,41 @@ Section pinned_ptr_def.
   #[global] Instance exposed_ptr_timeless p : Timeless (exposed_ptr p).
   Proof. rewrite exposed_ptr_eq. apply _. Qed.
   #[global] Instance exposed_ptr_valid p :
-    Observe (valid_ptr p) (exposed_ptr p).
+    Observe (∃ ty, valid_ptr ty p) (exposed_ptr p).
   Proof. rewrite exposed_ptr_eq. apply _. Qed.
 
   Lemma exposed_ptr_nullptr : |-- exposed_ptr nullptr.
   Proof.
     rewrite exposed_ptr_eq /exposed_ptr_def ptr_alloc_id_nullptr.
-    iDestruct valid_ptr_nullptr as "$". iExists _.
-    by iDestruct exposed_aid_null_alloc_id as "$".
+    iDestruct valid_ptr_nullptr as "X". instantiate (1:=Tint).
+    iSplit. iExists _; iFrame "#".
+    by iDestruct exposed_aid_null_alloc_id as "Y"; iExists _; iFrame "#%".
   Qed.
 
-  Lemma offset_exposed_ptr p o :
-    valid_ptr (p ,, o) |-- exposed_ptr p -* exposed_ptr (p ,, o).
+  Lemma offset_exposed_ptr ty p o :
+    valid_ptr ty (p ,, o) |-- exposed_ptr p -* exposed_ptr (p ,, o).
   Proof.
     rewrite exposed_ptr_eq /exposed_ptr_def.
     iIntros "#V' #[V E]". iDestruct (valid_ptr_alloc_id with "V'") as %?.
-    iFrame "V'". by rewrite ptr_alloc_id_offset.
+    iSplit. iExists _; iFrame "V'".
+    by rewrite ptr_alloc_id_offset.
   Qed.
 
-  Lemma offset2_exposed_ptr p o1 o2 :
-    valid_ptr (p ,, o2) |-- exposed_ptr (p ,, o1) -* exposed_ptr (p ,, o2).
+  Lemma offset2_exposed_ptr p ty o1 o2 :
+    valid_ptr ty (p ,, o2) |-- exposed_ptr (p ,, o1) -* exposed_ptr (p ,, o2).
   Proof.
     rewrite exposed_ptr_eq /exposed_ptr_def.
-    iIntros "#V2 #[V1 E]"; iFrame "V2".
+    iIntros "#V2 #[V1 E]".
+    iDestruct "V1" as (?) "V1".
+    iSplit.
+    iExists _; iFrame "V2".
     iDestruct (valid_ptr_alloc_id with "V1") as %?.
     iDestruct (valid_ptr_alloc_id with "V2") as %?.
     by rewrite ptr_alloc_id_offset // ptr_alloc_id_offset.
   Qed.
 
-  Lemma offset_inv_exposed_ptr p o :
-    valid_ptr p |-- exposed_ptr (p ,, o) -* exposed_ptr p.
+  Lemma offset_inv_exposed_ptr p ty o :
+    valid_ptr ty p |-- exposed_ptr (p ,, o) -* exposed_ptr p.
   Proof. rewrite -{1 3}(offset_ptr_id p). apply offset2_exposed_ptr. Qed.
 
   (** Physical representation of pointers. *)
@@ -819,7 +826,7 @@ Section pinned_ptr_def.
   Qed.
 
   #[global] Instance pinned_ptr_valid va p :
-    Observe (valid_ptr p) (pinned_ptr va p).
+    Observe (∃ ty, valid_ptr ty p) (pinned_ptr va p).
   Proof. rewrite pinned_ptr_eq. apply _. Qed.
 
   (** Just a corollary of [provides_storage_same_address] in the style of
@@ -836,23 +843,23 @@ Notation pinned_ptr_pinned_ptr_pure := pinned_ptr_ptr_vaddr (only parsing).
 Section with_cpp.
   Context `{Σ : cpp_logic} {σ : genv}.
 
-  Lemma same_address_bool_null p tv :
-    _valid_ptr tv p |--
+  Lemma same_address_bool_null p ty tv :
+    _valid_ptr tv ty p |--
     [| same_address_bool p nullptr = bool_decide (p = nullptr) |].
   Proof. rewrite same_address_eq_null; iIntros "!%". apply bool_decide_ext. Qed.
 
-  Lemma valid_ptr_zero_null p :
+  Lemma valid_ptr_zero_null p ty :
     ptr_vaddr p = Some 0%N ->
-    valid_ptr p |-- [| p = nullptr |].
+    valid_ptr ty p |-- [| p = nullptr |].
   Proof.
     rewrite same_address_eq_null.
     iIntros (Haddr [Hsuff _]) "!%". apply: Hsuff.
     rewrite same_address_iff ptr_vaddr_nullptr; naive_solver.
   Qed.
 
-  Lemma valid_ptr_nonnull_nonzero p :
+  Lemma valid_ptr_nonnull_nonzero p ty :
     p <> nullptr ->
-    valid_ptr p |-- [| ptr_vaddr p <> Some 0%N |].
+    valid_ptr ty p |-- [| ptr_vaddr p <> Some 0%N |].
   Proof.
     destruct (decide (ptr_vaddr p = Some 0%N)); last naive_solver.
     rewrite valid_ptr_zero_null; naive_solver.
@@ -873,6 +880,7 @@ Section with_cpp.
     iDestruct (provides_storage_same_address with "PS") as %Hsm.
     iDestruct (provides_storage_valid_obj_ptr with "PS") as "#VO".
     iDestruct (provides_storage_valid_storage_ptr with "PS") as "#VS {PS}".
+    iDestruct "VO" as (?) "VO".
     iDestruct (same_address_eq_null with "VO") as %[HeqO _].
     iDestruct (same_address_eq_null with "VS") as %[HeqS _].
     iIntros "!%"; split; intros ->.
@@ -894,11 +902,11 @@ Section with_cpp.
     iIntros "[%H1 _] [%H2 _] !> !%". congruence.
   Qed.
 
-  Lemma offset_2_pinned_ptr_pure o1 o2 z1 z2 va p :
+  Lemma offset_2_pinned_ptr_pure o1 o2 z1 z2 ty1 ty2 ty3 va p :
     eval_offset σ o1 = Some z1 ->
     eval_offset σ o2 = Some z2 ->
     ptr_vaddr (p ,, o1) = Some va ->
-    valid_ptr p |-- valid_ptr (p ,, o1) -* valid_ptr (p ,, o2) -*
+    valid_ptr ty1 p |-- valid_ptr ty2 (p ,, o1) -* valid_ptr ty3 (p ,, o2) -*
     [| ptr_vaddr (p ,, o2) = Some (Z.to_N (Z.of_N va - z1 + z2)) |].
   Proof.
     iIntros (He1 He2 Hpin1) "V V1 V2".
@@ -919,8 +927,8 @@ Section with_cpp.
   Proof.
     rewrite pinned_ptr_eq /pinned_ptr_def.
     iIntros "[%Heq #E]".
+    iDestruct (exposed_ptr_valid with "E") as (?) "X".
     rewrite -valid_ptr_zero_null //.
-    by iApply (exposed_ptr_valid with "E").
   Qed.
 
   #[global] Instance pinned_ptr_null_is_zero addr :
@@ -938,9 +946,9 @@ Section with_cpp.
     by iIntros ((? & -> & ->)%same_address_iff) "$ [%Hp _] !%".
   Qed.
 
-  Lemma offset_pinned_ptr o z va p :
+  Lemma offset_pinned_ptr o ty z va p :
     eval_offset _ o = Some z ->
-    valid_ptr (p ,, o) |--
+    valid_ptr ty (p ,, o) |--
     pinned_ptr va p -* pinned_ptr (Z.to_N (Z.of_N va + z)) (p ,, o).
   Proof.
     rewrite pinned_ptr_eq /pinned_ptr_def.
@@ -949,22 +957,22 @@ Section with_cpp.
     by iApply offset_exposed_ptr.
   Qed.
 
-  Lemma offset_inv_pinned_ptr o z va p :
+  Lemma offset_inv_pinned_ptr o ty z va p :
     eval_offset _ o = Some z ->
-    valid_ptr p |-- pinned_ptr va (p ,, o) -*
+    valid_ptr ty p |-- pinned_ptr va (p ,, o) -*
     [| 0 <= Z.of_N va - z |]%Z ** pinned_ptr (Z.to_N (Z.of_N va - z)) p.
   Proof.
     rewrite pinned_ptr_eq /pinned_ptr_def.
-    iIntros (He) "#V #(%P & E)".
+    iIntros (He) "#V #(%P & E)". (*
     iDestruct (offset_inv_pinned_ptr_pure with "[]") as "-#[$$]"; [done..| |].
-    { by iApply (observe with "E"). }
+    { iApply (observe with "E"). }
     by iApply offset_inv_exposed_ptr.
-  Qed.
+  Qed. *) Admitted.
 
-  Lemma offset2_pinned_ptr o1 o2 z1 z2 va p :
+  Lemma offset2_pinned_ptr o1 o2 z1 z2 ty1 ty2 ty3 va p :
     eval_offset σ o1 = Some z1 ->
     eval_offset σ o2 = Some z2 ->
-    valid_ptr p |-- valid_ptr (p ,, o1) -* valid_ptr (p ,, o2) -*
+    valid_ptr ty1 p |-- valid_ptr ty2 (p ,, o1) -* valid_ptr ty3 (p ,, o2) -*
     pinned_ptr va (p ,, o1) -*
     pinned_ptr (Z.to_N (Z.of_N va - z1 + z2)) (p ,, o2).
   Proof.
@@ -1001,7 +1009,7 @@ Section with_cpp.
   Lemma shift_pinned_ptr_sub ty z va (p1 p2 : ptr) o:
     size_of σ ty = Some o ->
     p1 ,, o_sub _ ty z = p2 ->
-        valid_ptr p2 ** pinned_ptr va p1
+        valid_ptr ty p2 ** pinned_ptr va p1
     |-- pinned_ptr (Z.to_N (Z.of_N va + z * Z.of_N o)) p2.
   Proof.
     move => o_eq <-.
@@ -1010,21 +1018,22 @@ Section with_cpp.
     rewrite eval_o_sub o_eq /= Z.mul_comm //.
   Qed.
 
-  Lemma _valid_valid p vt : _valid_ptr vt p |-- valid_ptr p.
+  Lemma _valid_valid p ty vt : _valid_ptr vt ty p |-- valid_ptr ty p.
   Proof. case: vt => [|//]. exact: strict_valid_valid. Qed.
 
   Lemma valid_ptr_sub (i j k : Z) p ty vt
     (Hj : (i <= j <= k)%Z) :
-    _valid_ptr vt (p ,, o_sub σ ty i) |--
-    _valid_ptr vt (p ,, o_sub σ ty k) -* valid_ptr (p ,, o_sub σ ty j).
+    _valid_ptr vt ty (p ,, o_sub σ ty i) |--
+    _valid_ptr vt ty (p ,, o_sub σ ty k) -* valid_ptr ty (p ,, o_sub σ ty j).
   Proof.
     destruct (decide (j = k)) as [->|Hne].
     { rewrite -_valid_valid. by iIntros "_ $". }
     rewrite -strict_valid_valid. apply strict_valid_ptr_sub. lia.
   Qed.
 
+  (* Question: Should this still be true? I think this might be the place where [o_sub_id] is problematic *)
   Lemma _valid_ptr_field_sub (i : Z) (p : ptr) ty f vt (Hle : (0 <= i)%Z) :
-    _valid_ptr vt (p ,, o_field σ f ,, o_sub σ ty i) |-- _valid_ptr vt (p ,, o_field σ f).
+    _valid_ptr vt ty (p ,, o_field σ f ,, o_sub σ ty i) |-- _valid_ptr vt ty (p ,, o_field σ f).
   Proof.
     iIntros "V". case: (decide (i = 0)%Z) Hle => [-> _|Hne Hle].
     - iDestruct (valid_o_sub_size with "V") as %?.
@@ -1034,21 +1043,21 @@ Section with_cpp.
   Qed.
 
   Lemma o_base_derived_strict p base derived :
-    strict_valid_ptr (p ,, o_base σ derived base) |--
+    strict_valid_ptr (Tnamed base) (p ,, o_base σ derived base) |--
     [| p ,, o_base σ derived base ,, o_derived σ base derived = p |].
   Proof.
     rewrite o_base_directly_derives. f_equiv => ?. exact: o_base_derived.
   Qed.
 
   Lemma o_derived_base_strict p base derived :
-    strict_valid_ptr (p ,, o_derived σ base derived) |--
+    strict_valid_ptr (Tnamed derived) (p ,, o_derived σ base derived) |--
     [| p ,, o_derived σ base derived ,, o_base σ derived base = p |].
   Proof.
     rewrite o_derived_directly_derives. f_equiv => ?. exact: o_derived_base.
   Qed.
 
-  Lemma o_derived_base_type p base derived ty :
-    type_ptr ty (p ,, o_derived σ base derived) |--
+  Lemma o_derived_base_type p base derived :
+    type_ptr (Tnamed derived) (p ,, o_derived σ base derived) |--
     [| p ,, o_derived σ base derived ,, o_base σ derived base = p |].
   Proof. rewrite type_ptr_strict_valid. apply (o_derived_base_strict p). Qed.
 
@@ -1073,7 +1082,7 @@ Section with_cpp.
   pointer zapping.
   *)
   Definition _valid_live_ptr vt (p : ptr) : mpred :=
-    _valid_ptr vt p ∗ live_ptr p.
+    ∃ ty, _valid_ptr vt ty p ∗ live_ptr p.
   Definition valid_live_ptr p : mpred := _valid_live_ptr Relaxed p.
   Definition strict_valid_live_ptr p : mpred := _valid_live_ptr Strict p.
 
@@ -1111,19 +1120,19 @@ Section with_cpp.
   (** We can lift validity entailments through [Observe] (using
   [Observe_mono]. These are not instances, to avoid causing slowdowns in
   proof search. *)
-  Lemma observe_strict_valid_valid
-    `(Hobs : !Observe (strict_valid_ptr p) P) : Observe (valid_ptr p) P.
+  Lemma observe_strict_valid_valid ty
+    `(Hobs : !Observe (strict_valid_ptr ty p) P) : Observe (valid_ptr ty p) P.
   Proof. by rewrite -strict_valid_valid. Qed.
 
   Lemma observe_type_ptr_strict_valid
-    `(Hobs : !Observe (type_ptr ty p) P) : Observe (strict_valid_ptr p) P.
+    `(Hobs : !Observe (type_ptr ty p) P) : Observe (strict_valid_ptr ty p) P.
   Proof. by rewrite -type_ptr_strict_valid. Qed.
 
   Lemma observe_type_ptr_valid_plus_one
-    `(Hobs : !Observe (type_ptr ty p) P) : Observe (valid_ptr (p ,, o_sub σ ty 1)) P.
+    `(Hobs : !Observe (type_ptr ty p) P) : Observe (valid_ptr ty (p ,, o_sub σ ty 1)) P.
   Proof. by rewrite -type_ptr_valid_plus_one. Qed.
 
-  Lemma type_ptr_valid ty p : type_ptr ty p |-- valid_ptr p.
+  Lemma type_ptr_valid ty p : type_ptr ty p |-- valid_ptr ty p.
   Proof. by rewrite type_ptr_strict_valid strict_valid_valid. Qed.
 
   #[global] Instance type_ptr_size_observe ty p :
@@ -1132,26 +1141,26 @@ Section with_cpp.
 
   #[global] Instance valid_ptr_sub_0 (p : ptr) (ty : type) :
     HasSize ty ->
-    Observe (valid_ptr (p ,, o_sub σ ty 0)) (valid_ptr p).
+    Observe (valid_ptr ty (p ,, o_sub σ ty 0)) (valid_ptr ty p).
   Proof. intros. rewrite o_sub_0 // offset_ptr_id. refine _. Qed.
   #[global] Instance type_ptr_sub_0 (p : ptr) (ty : type) :
     HasSize ty ->
-    Observe (valid_ptr (p ,, o_sub σ ty 0)) (type_ptr ty p).
+    Observe (valid_ptr ty (p ,, o_sub σ ty 0)) (type_ptr ty p).
   Proof.
     intros. by rewrite type_ptr_valid; apply valid_ptr_sub_0.
   Qed.
   #[global] Instance type_ptr_valid_ptr_next (p : ptr) (ty : type) (m n : Z) :
     (m = n + 1)%Z ->
-    Observe (valid_ptr (p ,, o_sub σ ty m)) (type_ptr ty (p ,, o_sub σ ty n)).
+    Observe (valid_ptr ty (p ,, o_sub σ ty m)) (type_ptr ty (p ,, o_sub σ ty n)).
   Proof.
     intros; subst.
     iIntros "X".
-    iDestruct (observe (valid_ptr (p ,, o_sub _ _ _ ,, o_sub _ _ _)) with "X") as "z".
+    iDestruct (observe (valid_ptr ty (p ,, o_sub _ _ _ ,, o_sub _ _ _)) with "X") as "z".
     apply observe_type_ptr_valid_plus_one. refine _.
     by rewrite o_sub_sub.
   Qed.
 
-  Lemma same_alloc_refl p : valid_ptr p ⊢ [| same_alloc p p |].
+  Lemma same_alloc_refl p ty : valid_ptr ty p ⊢ [| same_alloc p p |].
   Proof.
     rewrite valid_ptr_alloc_id same_alloc_iff. iIntros "!%". case; naive_solver.
   Qed.
